try to write some test.

ass1/Ex6.dfy
@@ -1,5 +1,11 @@
+predicate Clean(a: array<int>, key: int) 
+    reads a 
+{
+    forall k ::0<= k < a.Length ==> a[k] != key
+}
+
 method IsClean(a: array<int>, key: int) returns (clean: bool) 
-    ensures clean <==> forall k ::  0<= k < a.Length ==> a[k] != key
+    ensures clean <==> Clean(a,key)
 {
     clean := true ;
     var i := 0;
@@ -20,17 +26,31 @@ method IsClean(a: array<int>, key: int) returns (clean: bool)
 }
 
 
-method Test(){
-    var a:= new int[5];
-    a[0] := 1;
-    a[1] := 2;
-    a[2] := 2;
-    a[3] := 2;
-    a[4] := 3;
-    var b:=  IsClean(a, 1);
-    assert b;
-    b:= IsClean(a, 2);
-    assert b;
-    b:= IsClean(a, 3);
-    assert b;
-}
+    method Test(){
+        var a:= new int[5][1,2,2,2,3];
+        assert a[0] == 1;
+        assert a[1] == 2;
+        assert a[2] == 2;
+        assert a[3] == 2;
+        assert a[4] == 3;
+
+        var b:=  IsClean(a, 5);
+        assert b==true;
+        b:= IsClean(a, 2);
+        assert !b;
+        b:= IsClean(a, 3);
+        assert !b;
+        b:= IsClean(a, 4);
+        assert b;
+
+        var c:= new int[1][1];
+        assert c[0]== 1;
+        b:= IsClean(c,1);
+        assert !b;
+        b:= IsClean(c,2);
+        assert b;
+
+        var d:= new int[0][];
+        b:= IsClean(d,1);
+        assert b;
+    }
